

## Chapter2 Bernoulli Trials

Below  $S_n$  denotes the total number of successes, and has the binomial distribution with parameters  $n$  and  $p$ .

### *Bernoulli's law of Large Number*

$p$  does not depend on  $n$ , then for any  $\epsilon > 0$

$$\lim_{n \rightarrow \infty} P \left\{ \left| \frac{S_n}{n} - p \right| > \epsilon \right\} = 0$$

It follows at once from Chebyshev's inequality

### *Chebyshev's inequality*

For all  $n > 0, \epsilon > 0$

$$P \{ |S_n - np| > n\epsilon \} \leq \frac{p(1-p)}{n\epsilon^2}$$

proof:

$$\begin{aligned} P \{ |S_n - np| > n\epsilon \} &= \sum_{0 \leq k \leq n, |k - np| > n\epsilon} \binom{n}{k} p^k (1-p)^{n-k} \\ &\leq \sum_{0 \leq k \leq n, |k - np| > n\epsilon} \left( \frac{k - np}{n\epsilon} \right)^2 \binom{n}{k} p^k (1-p)^{n-k} \\ &\leq \frac{1}{(n\epsilon)^2} \sum_{k=0}^n (k - np)^2 \binom{n}{k} p^k (1-p)^{n-k} \\ &= \frac{\text{var} S_n}{(n\epsilon)^2} = \frac{p(1-p)}{n\epsilon^2} \end{aligned}$$

### *The de Moivre-Laplace Central Limit Theorem*

$p$  does not depend on  $n$ , then for all finite numbers  $a < b$ ,

$$\lim_{n \rightarrow \infty} P \left\{ a < \frac{S_n - np}{\sqrt{np(1-p)}} \leq b \right\} = P \{ a < N(0, 1) \leq b \}$$

to estimate  $\binom{n}{k}$ , we only need to estimate  $k!$  for all  $k$ . Then we have result below

### *de Moivre's Formula*

There exists  $\beta \in (0, +\infty)$  such that

$$n! \sim \beta n^{n+1/2} e^{-n} \quad \text{as } n \rightarrow \infty$$

proof:

define:  $f(n) = \frac{n!}{\beta n^{n+1/2} e^{-n}}$

$f(1) = e$ , then we can write  $f(n)$  as

$$f(n) = e \prod_{k=2}^n \frac{f(k)}{f(k-1)} = \exp \left\{ 1 + \sum_{k=2}^n \ln f(k) - \ln f(k-1) \right\}$$

as  $k \rightarrow \infty$ ,

$$\ln f(k) - \ln f(k-1) = 1 + \left(k - \frac{1}{2}\right) \ln \left(1 - \frac{1}{k}\right) \sim -\frac{1}{12k^2}$$

since

$$\sum_{k=2}^{\infty} \ln f(k) - \ln f(k-1) < \infty$$

we have the result.

proof of The de Moivre-Laplace CLT:

let  $q = 1 - p$

$$\begin{aligned} P \left\{ a < \frac{Sn - np}{\sqrt{np(1-p)}} \leq b \right\} &= \sum_{np + a\sqrt{npq} < k \leq np + b\sqrt{npq}} \binom{n}{k} p^k q^{n-k} \\ &= \sum_{a\sqrt{npq} < \lambda \leq b\sqrt{npq}} \binom{n}{\lambda + np} p^{\lambda + np} q^{nq - k} \end{aligned}$$

The index  $k$  is in  $\{0, \dots, n\}$ , while  $\lambda$  runs over all real numbers of the form  $k - np$ ,

let us call any  $\lambda$  of this form an  $n - \text{admissible}$  number.

According to the de Moivre's Formula:

as  $n \rightarrow \infty$ :

$$\binom{n}{\lambda + np} \sim \frac{1}{\beta \sqrt{npq}} \left( \frac{\lambda}{n} + p \right)^{-\lambda - np} \left( q - \frac{\lambda}{n} \right)^{-nq + \lambda}$$

for all  $n - \text{admissible}$  number  $\lambda \in [a\sqrt{npq}, b\sqrt{npq}]$

Thus as  $n \rightarrow \infty$ :

$$P \left\{ a < \frac{Sn - np}{\sqrt{np(1-p)}} \leq b \right\} \sim \frac{1}{\beta \sqrt{npq}} \sum_{a\sqrt{npq} < \lambda \leq b\sqrt{npq}} \left( \frac{\lambda}{n} + p \right)^{-\lambda - np} \left( q - \frac{\lambda}{n} \right)^{-nq + \lambda}$$

since as  $n \rightarrow \infty$ :

$$\left(\frac{\lambda}{n} + p\right)^{-\lambda-np} \left(q - \frac{\lambda}{n}\right)^{-nq+\lambda} \sim e^{-\lambda^2/2npq}$$

and by the definition of Riemann integrals:

$$P \left\{ a < \frac{Sn - np}{\sqrt{np(1-p)}} \leq b \right\} \sim \frac{1}{\beta\sqrt{npq}} \int_{a\sqrt{npq}}^{b\sqrt{npq}} e^{-x^2/2npq} dx$$

that is

$$\lim_{n \rightarrow \infty} P \left\{ a < \frac{Sn - np}{\sqrt{np(1-p)}} \leq b \right\} = \int_a^b \frac{e^{-\frac{x^2}{2}}}{\beta} dx = \frac{\sqrt{2\pi}}{\beta} \int_a^b \phi(x) dx$$

$\phi(x)$  demotes the standard-normal density function.

we then proof that  $\beta = \sqrt{2\pi}$

By chebyshev's inequality:

$$1 \geq P \left\{ -a < \frac{Sn - np}{\sqrt{np(1-p)}} \leq a \right\} \geq 1 - \frac{1}{a^2}$$

for all  $n > 0, a > 0$

let  $n \rightarrow \infty$ :

$$\frac{\beta}{\sqrt{2\pi}} \geq \int_{-a}^a \phi(x) dx \geq \frac{\beta}{\sqrt{2\pi}} \left(1 - \frac{1}{a^2}\right)$$

let  $a \rightarrow \infty$ :

$$\int_{-\infty}^{\infty} \phi(x) dx = \frac{\beta}{\sqrt{2\pi}} = 1$$

thus  $\beta = \sqrt{2\pi}$

we verify that  $\beta = \sqrt{2\pi}$ , we have the Stirling formula:

**Stirling Formula:**

$$n! \sim n^{n+1/2} e^{-n} \sqrt{2\pi} \quad \text{as } n \rightarrow \infty$$